Added other types, and simplified definition of substitution on types

mechanization/comp_expr.v
@@ -1,22 +1,37 @@
 Require Import worlds.
+Require Import util.
 Require Import meta_term.
 Require Import meta_subst.
  
- Inductive tp (D:world) :=
-  | m_tp : mtype D -> tp D
-  | arr : tp D -> tp D -> tp D
-  | prod : forall D2, wlink D D2 -> mtype D -> tp D2 -> tp D
+ Set Implicit Arguments.
+ Inductive tp' ψ (δ:world):=
+  | m_tp : mtype δ -> tp' ψ δ
+  | arr : tp' ψ δ -> tp' ψ δ -> tp' ψ δ
+  | pi : forall δ', δ↪δ' -> mtype δ -> tp' ψ δ' -> tp' ψ δ
+  | sigma : forall δ', δ↪δ' -> mtype δ -> tp' ψ δ' -> tp' ψ δ
+  | unit : tp' ψ δ
+  | prod : tp' ψ δ -> tp' ψ δ -> tp' ψ δ
+  | sum : tp' ψ δ -> tp' ψ δ -> tp' ψ δ
+(*  | mu : forall δ' ψ', star (fun δ1 δ2 => (mtype δ1)*(δ1↪δ2)) δ δ'
+         ->  ψ↪ψ'
+         -> tp' ψ' δ'
+         -> tp' ψ δ *)
+  | tvar : name ψ -> tp' ψ δ
+  | tapp : tp' ψ δ -> meta_term δ -> tp' ψ δ
+  | eq_constraint : meta_term δ -> meta_term δ -> tp' ψ δ -> tp' ψ δ
  .
- Coercion m_tp : mtype >-> tp.
- Implicit Arguments m_tp.
- Implicit Arguments arr.
- Implicit Arguments prod.
+
+ Definition tp δ := tp' empty δ.
+ Unset Implicit Arguments.
+ Definition m_tp' {δ} := @m_tp empty δ : mtype δ -> tp δ.
+ Coercion m_tp' : mtype >-> tp.
 
  Inductive synth_exp (D G:world) : Set :=
   | var : name G -> synth_exp D G
   | app :  synth_exp D G -> checked_exp D G -> synth_exp D G
   | mapp : synth_exp D G -> meta_term D -> synth_exp D G
   | coercion : checked_exp D G -> tp D -> synth_exp D G
+  | unfold : synth_exp D G -> synth_exp D G
  with checked_exp (D G:world) : Set := 
   | synth : synth_exp D G -> checked_exp D G
   | meta : meta_term D -> checked_exp D G
@@ -25,6 +40,12 @@ Require Import meta_subst.
   | case_i :  synth_exp D G -> list (branch D G) -> checked_exp D G
   | case_c : meta_term D -> list (branch D G) -> checked_exp D G
   | rec : forall G2, wlink G G2 -> checked_exp D G2 -> checked_exp D G
+  | fold : checked_exp D G -> checked_exp D G
+  | inl : checked_exp D G -> checked_exp D G
+  | inr : checked_exp D G -> checked_exp D G
+  | pack : meta_term D -> checked_exp D G -> checked_exp D G
+  | pair : checked_exp D G -> checked_exp D G -> checked_exp D G
+  | tt : checked_exp D G
  with branch (D G:world) : Set :=
   | br : forall Di, meta_term Di -> msubst D Di -> checked_exp Di G -> branch D G.
  Coercion synth : synth_exp >-> checked_exp.
