meta_subst_type.v
@@ -1,28 +1,48 @@
+Require Import util.
 Require Import worlds.
 Require Import meta_subst.
 Require Import comp_expr.
 Require Import meta_subst_meta_type.
-
+Require Import meta_subst_meta_term.
+Require Import meta_subst_typing.
+Require Import meta_term.
 Axiom theta_weaken : forall {D R} (theta:msubst D R) {R'} (X:wlink R R'), msubst D R'.
 
-Definition app_msubst_t2' : forall {W} (T:tp W) {W'} (theta:msubst W W'), tp W'.
-induction 1; intros.
-apply m_tp.
-eapply app_msubst_t. eexact theta. exact m.
-apply arr. apply IHT1. exact theta. apply IHT2. exact theta.
-Print Implicit prod.
-Print projT1.
-apply (prod (projT2 (next W'))).
-eapply app_msubst_t. eexact theta. eexact m.
-apply IHT.
-econstructor. eapply theta_weaken. eexact theta.
-eexact (projT2 (next W')).
-split. eexact w. constructor 3. eapply (weaken (projT2 (next W'))).
-Defined.
 
-Definition app_msubst_t2 {W W'} (theta:msubst W W') (T:tp W) : tp W' := app_msubst_t2' T theta.
+Section app_msubst_t2_sect.
+
+Notation "θ ;; X' // X" := ((theta_weaken θ X') ; (m_var X') // X) (at level 90).
+Reserved Notation "[ θ ] T" (at level 90).
+
+Fixpoint app_msubst_t2 {ψ} {δ δ'} (θ:msubst δ δ') (T:tp' ψ δ) : tp' ψ δ' :=
+match T  with
+ | m_tp U     =>
+   m_tp _ (⟦θ⟧ U)
+ | arr T1 T2  =>
+   arr ([θ] T1) ([θ] T2)
+ | pi _ X U T0 =>
+   let (_,X') := next δ' in
+   pi X' (⟦θ⟧ U) ([θ;;X'//X] T0)
+ | sigma _ X U T0 =>
+   let (_,X') := next δ' in
+   sigma X' (⟦θ⟧ U) ([θ;;X'//X] T0)
+ | unit =>
+   unit _ _
+ | prod T1 T2 =>
+   prod ([θ] T1) ([θ] T2)
+ | sum T1 T2 =>
+   sum ([θ] T1) ([θ] T2)
+ | tvar n =>
+   tvar _ n
+ | tapp T0 C =>
+   tapp ([θ] T0) (⟦θ⟧ C)
+ | eq_constraint C1 C2 T0 =>
+   eq_constraint (⟦θ⟧ C1) (⟦θ⟧ C2) ([θ] T0)
+end
+where "[ θ ] T" := (app_msubst_t2 θ T).
+End app_msubst_t2_sect.
 Implicit Arguments app_msubst_t2.
-Require Import meta_term.
+
 
 Axiom msubst_single_t : forall {D D'} (X:wlink D D'), meta_term D -> tp D' -> tp D.
 (* TODO: Write this as a simultaneous substitution: (id,C/X) ? *)
